Proper trace semantics with worked examples

TraceSemantics.v
@@ -28,15 +28,6 @@ Open Scope trace_scope.
 
 (** Symbolic semantics *)
 
-(** How should a /trace/ keep track of the current stack frame? *)
-
-(* keep the substitutions around? feels cheat-y *)
-(* record "procedure call" in the trace? *)
-(* inline the procedure body like in OOP.v? <-- easier implementation? *)
-(* continuations like in LAGC? <-- probably better suited to parallelism *)
-
-(** last two both seem reasonable, but lets try the easiest *)
-
 Fixpoint Stmt_sub (s:Stmt) (u y:LVar) : Stmt :=
   let t : LSub := (u !-> (ALVar y) ; Lid_sub) in
   match s with
@@ -49,7 +40,6 @@ Fixpoint Stmt_sub (s:Stmt) (u y:LVar) : Stmt :=
   | SReturn => SReturn
   end.
 
-
 Definition STrace_step : Type := (Bexpr + (GVar * Aexpr) + (LVar * Aexpr)).
 
 Definition cond  : Bexpr -> STrace_step := fun x => inl (inl x).
@@ -58,27 +48,46 @@ Definition asgnL : LVar -> Aexpr -> STrace_step := fun x e => inr (x, e).
 
 Definition STrace := trace STrace_step.
 
+Fixpoint acc_GSubst (G:GSub) (L:LSub) (t:STrace) : GSub :=
+  match t with
+  | [] => G
+  | t' :: inl (inr (x, e)) => update (acc_GSubst G L t') x (Aapply (acc_GSubst G L t') (acc_LSubst G L t') e)
+  | t' :: _ => acc_GSubst G L t'
+  end
+with acc_LSubst (G:GSub) (L:LSub) (t:STrace) : LSub :=
+  match t with
+  | [] => L
+  | t' :: inr (x, e) => update (acc_LSubst G L t') x (Aapply (acc_GSubst G L t') (acc_LSubst G L t') e)
+  | t' :: _ => acc_LSubst G L t'
+  end.
+
+Definition Aapply_t : STrace -> Aexpr -> Aexpr :=
+fun t e => Aapply (acc_GSubst Gid_sub Lid_sub t) (acc_LSubst Gid_sub Lid_sub t) e.
+
+Definition Bapply_t : STrace -> Bexpr -> Bexpr :=
+fun t e => Bapply (acc_GSubst Gid_sub Lid_sub t) (acc_LSubst Gid_sub Lid_sub t) e.
+
 Definition SConfig : Type := Stmt * STrace.
 
 Reserved Notation " c '->s' c' " (at level 40).
 Inductive Sstep : relation SConfig  :=
 | SGAsgn_step : forall x e s t,
-    (<{ x :=G e ; s }>, t) ->s (s, (t :: asgnG x e))
+    (<{ x :=G e ; s }>, t) ->s (s, (t :: asgnG x (Aapply_t t e)))
 | SLAsgn_step : forall x e s t,
-    (<{ x :=L e ; s }>, t) ->s (s, t :: asgnL x e)
+    (<{ x :=L e ; s }>, t) ->s (s, t :: asgnL x (Aapply_t t e))
 | SProc_step : forall (t:STrace) u y body e s t,
     (* "y fresh", somehow *)
-    (<{ proc(u){body}(e) ; s }>, t) ->s (SSeq (Stmt_sub body u y) s, t :: asgnL y e)
+    (<{ proc(u){body}(e) ; s }>, t) ->s (SSeq (Stmt_sub body u y) s, t :: asgnL y (Aapply_t t e))
 | SReturn_step : forall s t,
     (<{ return ; s }>, t) ->s (s, t)
 | SIfTrue_step : forall b s1 s2 s t,
-    (<{ if b {s1}{s2} ; s}>, t) ->s (<{ s1 ; s }>, t :: cond  b)
+    (<{ if b {s1}{s2} ; s}>, t) ->s (<{ s1 ; s }>, t :: cond  (Bapply_t t b))
 | SIfFalse_step : forall b s1 s2 s t,
-    (<{ if b {s1}{s2} ; s}>, t) ->s (<{ s2 ; s }>, t :: cond  (BNot b))
+    (<{ if b {s1}{s2} ; s}>, t) ->s (<{ s2 ; s }>, t :: cond  (BNot (Bapply_t t b)))
 | SWhileTrue_step : forall b s s' t,
-    (<{ while b {s} ; s' }>, t) ->s (<{ s ; while b {s} ; s' }>, t :: cond  b)
+    (<{ while b {s} ; s' }>, t) ->s (<{ s ; while b {s} ; s' }>, t :: cond  (Bapply_t t b))
 | SWhileFalse_step : forall b s s' t,
-    (<{ while b {s} ; s' }>, t) ->s (s', t :: cond  (BNot b))
+    (<{ while b {s} ; s' }>, t) ->s (s', t :: cond  (BNot (Bapply_t t b)))
   where " c '->s' c' " := (Sstep c c').
 
 Definition multi_Sstep := clos_refl_trans_n1 _ Sstep.
@@ -91,51 +100,56 @@ Definition CTrace_step : Type := (GVar * Val) + (LVar * Val).
 
 Definition CTrace := trace CTrace_step.
 
-(* for now, let's just "cheat" in totality *)
-Fixpoint acc_GVal (t:CTrace) : GVal :=
+Fixpoint acc_GVal (G0:GVal) (L0:LVal) (t:CTrace) : GVal :=
   match t with
-  | Tnil => (_ !-> 0)
-  | Tcons t' (inr _) => acc_GVal t'
-  | Tcons t' (inl (x, e)) => update (acc_GVal t') x e
+  | Tnil => G0
+  | Tcons t' (inr _) => acc_GVal G0 L0 t'
+  | Tcons t' (inl (x, e)) => let G' := acc_GVal G0 L0 t' in
+                            let L' := acc_LVal G0 L0 t' in update G' x (Aeval G' L' e)
+  end
+with acc_LVal (G0:GVal) (L0:LVal) (t:CTrace) : LVal :=
+  match t with
+  | Tnil => L0
+  | Tcons t' (inl _) => acc_LVal G0 L0 t'
+  | Tcons t' (inr (x, e)) => let G' := acc_GVal G0 L0 t' in
+                            let L' := acc_LVal G0 L0 t' in update L' x (Aeval G' L' e)
   end.
 
-Fixpoint acc_LVal (t:CTrace) : LVal :=
-  match t with
-  | Tnil => (_ !-> 0)
-  | Tcons t' (inl _) => acc_LVal t'
-  | Tcons t' (inr (x, e)) => update (acc_LVal t') x e
-  end.
+Definition Aeval_t (G0:GVal) (L0:LVal) (t:CTrace) (e:Aexpr) : nat :=
+  Aeval (acc_GVal G0 L0 t) (acc_LVal G0 L0 t) e.
 
-Definition Aeval_t (t:CTrace) (e:Aexpr) : nat :=
-  Aeval (acc_GVal t) (acc_LVal t) e.
-
-Definition Beval_t (t:CTrace) (b:Bexpr) : bool :=
-  Beval (acc_GVal t) (acc_LVal t) b.
+Definition Beval_t (G0:GVal) (L0:LVal) (t:CTrace) (b:Bexpr) : bool :=
+  Beval (acc_GVal G0 L0 t) (acc_LVal G0 L0 t) b.
 
 Definition CConfig : Type := Stmt * CTrace.
 
 Reserved Notation " c '=>c' c' " (at level 40).
 
 Inductive Cstep : relation CConfig :=
-| CGAsgn_step : forall x e s t,
-    (<{ x :=G e ; s }>, t) =>c (s, t :: inl (x, Aeval_t t e))
-| CLAsgn_step : forall x e s t,
-    (<{ x :=L e ; s }>, t) =>c (s, t :: inr (x, Aeval_t t e))
-| CProc_step : forall u body e s t y,
-    (<{ proc(u){body}(e) ; s }>, t) =>c (SSeq (Stmt_sub body u y) s, t :: inr (y, Aeval_t t e))
+| CGAsgn_step : forall x e s t G0 L0 v,
+    Aeval_t G0 L0 t e = v ->
+    (<{ x :=G e ; s }>, t) =>c (s, t :: inl (x, v))
+| CLAsgn_step : forall x e s t G0 L0 v,
+    Aeval_t G0 L0 t e = v ->
+    (<{ x :=L e ; s }>, t) =>c (s, t :: inr (x, v))
+| CProc_step : forall u body e s s' t y G0 L0 v,
+    (* y fresh *)
+    Aeval_t G0 L0 t e = v ->
+    Stmt_sub body u y = s ->
+    (<{ proc(u){body}(e) ; s' }>, t) =>c (<{s ; s'}>, t :: inr (y, v))
 | CReturn_step : forall s t,
     (<{ return ; s }>, t) =>c (s, t)
-| CIfTrue_step : forall b s1 s2 s t,
-    Beval_t t b = true ->
+| CIfTrue_step : forall b s1 s2 s t G0 L0,
+    Beval_t G0 L0 t b = true ->
     (<{ if b {s1}{s2} ; s }>, t) =>c (<{s1 ; s}>, t)
-| CIfFalse_step : forall b s1 s2 s t,
-    Beval_t t b = false ->
+| CIfFalse_step : forall b s1 s2 s t G0 L0,
+    Beval_t G0 L0 t b = false ->
     (<{ if b {s1}{s2} ; s }>, t) =>c (<{s2 ; s}>, t)
-| CWhileTrue_step : forall b s s' t,
-    Beval_t t b = true ->
+| CWhileTrue_step : forall b s s' t G0 L0,
+    Beval_t G0 L0 t b = true ->
     (<{ while b {s} ; s' }>, t) =>c (<{s ; while b {s} ; s'}>, t)
-| CWhileFalse_step : forall b s s' t,
-    Beval_t t b = false ->
+| CWhileFalse_step : forall b s s' t G0 L0,
+    Beval_t G0 L0 t b = false ->
     (<{ while b {s} ; s' }>, t) =>c (s', t)
   where " c '=>c' c' " := (Cstep c c').
 
@@ -147,6 +161,10 @@ Notation " c '=>*' c' " := (multi_Cstep c c') (at level 40).
 Definition X : GVar := "X".
 Definition Y : LVar := "Y".
 Definition U : LVar := "U".
+
+(* not sure how to elegantly incorporate this assumption without semantics *)
+Axiom Seq_Assoc : forall s1 s2 s3,
+    <{ (s1 ; s2) ; s3 }> = <{ s1 ; s2 ; s3 }>.
 
 Example test_program : Stmt :=
   <{proc(U){ U :=L U + 1;
@@ -165,48 +183,53 @@ Lemma test_body_subst :
         U Y.
 Proof. simpl. rewrite L_single_update. reflexivity. Qed.
 
-(* not sure how to elegantly incorporate this assumption without semantics *)
-Lemma seq_assoc : forall s1 s2 s3,
-    <{(s1; s2); s3}> = <{s1 ; (s2 ; s3)}>. Admitted.
 
 Example Stest_trace : (test_program, [])
                         ->* (<{X :=G 0}>,
                                 [inr (Y, <{X + 1}>);
-                                  inr (Y, <{Y + 1}>);
-                                  inl (inr (X, <{Y + 2}>))]).
+                                  inr (Y, <{(X + 1) + 1}>);
+                                  inl (inr (X, <{(X + 1) + 1 + 2}>))]).
 Proof.
-  eapply Relation_Operators.rtn1_trans. apply SReturn_step.
-  eapply Relation_Operators.rtn1_trans. apply SGAsgn_step.
-  eapply Relation_Operators.rtn1_trans. apply SLAsgn_step.
-  eapply Relation_Operators.rtn1_trans.
-  assert (<{ Y :=L Y + 1; X :=G Y + 2; return; X :=G 0 }> = <{ (Y :=L Y + 1; X :=G Y + 2; return); X :=G 0 }>). {
-    repeat (rewrite seq_assoc). reflexivity. }
-  rewrite H. rewrite test_body_subst. apply SProc_step.
-  exact [].
-  apply rtn1_refl.
+  assert (step1 : (test_program, [])
+                  ->s (<{ (Y :=L Y + 1; X :=G Y + 2; return); X :=G 0 }>, [inr (Y, <{ X + 1 }>)])).
+  { rewrite test_body_subst. apply SProc_step. exact []. }
+  assert (step2 : (<{ Y :=L Y + 1; X :=G Y + 2; return; X :=G 0 }>, [inr (Y, <{ X + 1 }>)])
+                  ->s (<{ X :=G Y + 2; return; X :=G 0 }>, [inr (Y, <{ X + 1 }>)] :: inr (Y, <{ (X + 1) + 1 }>))).
+   { apply SLAsgn_step. }
+   assert (step3 : (<{ X :=G Y + 2; return; X :=G 0 }>, [inr (Y, <{ X + 1 }>) ; inr (Y, <{ (X + 1) + 1 }>)])
+          ->s (<{ return; X :=G 0 }>, [inr (Y, <{ X + 1 }>) ; inr (Y, <{ (X + 1) + 1 }>)] :: inl (inr (X, <{ ((X + 1) + 1) + 2 }>)))).
+   { apply SGAsgn_step. }
+   eapply Relation_Operators.rtn1_trans. apply SReturn_step.
+   eapply Relation_Operators.rtn1_trans. apply step3.
+   eapply Relation_Operators.rtn1_trans. apply step2.
+   assert (assoc : <{ (Y :=L Y + 1; X :=G Y + 2; return); X :=G 0 }> = <{ Y :=L Y + 1; X :=G Y + 2; return; X :=G 0 }>).
+   { repeat (rewrite Seq_Assoc). reflexivity. }
+   eapply Relation_Operators.rtn1_trans. rewrite <- assoc. apply step1.
+   apply rtn1_refl.
 Qed.
 
 Example Ctest_trace : (test_program, [])
-                        =>* (<{X :=G 0}>,
-                                [inr (Y, 1) ;
-                                  inr (Y, 2);
-                                 inl (X, 4)]).
+                        =>*  (<{X :=G 0}>,
+                                 [inr (Y, 1) ;
+                                   inr (Y, 2);
+                                   inl (X, 4)]).
 Proof.
-  eapply Relation_Operators.rtn1_trans. apply CReturn_step.
-  assert (step1 : (test_program, []) =>c (<{Y :=L Y + 1; X :=G Y + 2; return ; X :=G 0}>, [inr (Y, 1)])).
-  {assert (<{ Y :=L Y + 1; X :=G Y + 2; return; X :=G 0 }> = <{ (Y :=L Y + 1; X :=G Y + 2; return); X :=G 0 }>). {
-    repeat (rewrite seq_assoc). reflexivity. }
-    rewrite H. rewrite test_body_subst. apply CProc_step. }
-  assert (step2 : (<{Y :=L Y + 1; X :=G Y + 2; return ; X :=G 0}>, [inr (Y, 1)])
-          =>c (<{ X :=G Y + 2; return; X :=G 0}>, [inr (Y,1) ; inr (Y, 2)])).
-  { apply CLAsgn_step. }
-  assert (step3 : (<{ X :=G Y + 2; return; X :=G 0}>, [inr (Y,1) ; inr (Y, 2)])
-          =>c (<{return; X :=G 0}>, [inr (Y,1) ; inr (Y, 2) ; inl (X, 4)])).
-  { apply CGAsgn_step. }
-  eapply Relation_Operators.rtn1_trans. apply step3.
-  eapply Relation_Operators.rtn1_trans. apply step2.
-  eapply Relation_Operators.rtn1_trans. apply step1.
-  apply rtn1_refl.
+  assert (step1 : (test_program, [])
+                  =>c (<{ (Y :=L Y + 1; X :=G Y + 2; return); X :=G 0 }>, [inr (Y, 1)])).
+  { rewrite test_body_subst. apply CProc_step with (G0 := (_ !-> 0)) (L0 := (_ !-> 0)); reflexivity. }
+  assert (step2 : (<{ Y :=L Y + 1; X :=G Y + 2; return; X :=G 0 }>, [inr (Y, 1)])
+                  =>c (<{ X :=G Y + 2; return; X :=G 0 }>, [inr (Y, 1)] :: inr (Y, 2))).
+   { apply CLAsgn_step with (G0 := (_ !-> 0)) (L0 := (_ !-> 0)); reflexivity. }
+   assert (step3 : (<{ X :=G Y + 2; return; X :=G 0 }>, [inr (Y, 1) ; inr (Y, 2)])
+          =>c (<{ return; X :=G 0 }>, [inr (Y, 1) ; inr (Y, 2)] :: inl (X, 4))).
+   { apply CGAsgn_step with (G0 := (_ !-> 0)) (L0 := (_ !-> 0)); reflexivity. }
+   eapply Relation_Operators.rtn1_trans. apply CReturn_step.
+   eapply Relation_Operators.rtn1_trans. apply step3.
+   eapply Relation_Operators.rtn1_trans. apply step2.
+   assert (assoc : <{ (Y :=L Y + 1; X :=G Y + 2; return); X :=G 0 }> = <{ Y :=L Y + 1; X :=G Y + 2; return; X :=G 0 }>).
+   { repeat (rewrite Seq_Assoc). reflexivity. }
+   eapply Relation_Operators.rtn1_trans. rewrite <- assoc. apply step1.
+   apply rtn1_refl.
 Qed.
 
 (** Correctness *)
@@ -219,19 +242,28 @@ Fixpoint pc (t:STrace) : Bexpr :=
   | t' :: inl (inl p) => BAnd p (pc t')
   end.
 
-(*Cheated totality again*)
-Fixpoint acc_GSubst (t:STrace) : GSub :=
-  match t with
-  | [] => (_ !-> 0) (* this needs to be 0 to work with valuations*)
-  | t' :: inl (inr (x, e)) => update (acc_GSubst t') x (Aapply (acc_GSubst t') (acc_LSubst t') e)
-  | t' :: _ => acc_GSubst t'
-  end
-with acc_LSubst (t:STrace) : LSub :=
-  match t with
-  | [] => (_ !-> 0) (* this needs to be 0 to work with valuations*)
-  | t' :: inr (x, e) => update (acc_LSubst t') x (Aapply (acc_GSubst t') (acc_LSubst t') e)
-  | t' :: _ => acc_LSubst t'
-  end.
+Ltac splits := repeat (try split).
+
+Theorem correctness : forall s s' t G0 L0,
+    (s, []) ->* (s', t) ->
+    Beval G0 L0 (pc t) = true ->
+    exists t', (s, []) =>* (s', t')
+              /\ acc_GVal G0 L0 t' = GComp G0 L0 (acc_GSubst Gid_sub Lid_sub t)
+              /\ acc_LVal G0 L0 t' = LComp G0 L0 (acc_LSubst Gid_sub Lid_sub t).
+Proof.
+  intros. dependent induction H.
+  - exists []. splits. apply rtn1_refl.
+  - dependent destruction H.
+    + (* global assignment *)
+      destruct (IHclos_refl_trans_n1 s <{ x :=G e ; s'}> t0) as [t' [comp [IHG IHL]]];
+        try reflexivity;
+        try assumption.
+      exists (t' :: inl (x, Aeval_t (acc_GVal G0 L0 t') (acc_LVal G0 L0 t') t' e)). splits.
+      * eapply Relation_Operators.rtn1_trans. apply CGAsgn_step with (e := e) (G0 := acc_GVal G0 L0 t') (L0 := acc_LVal G0 L0 t').
+        reflexivity. assumption.
+      * simpl. unfold Aeval_t. rewrite Gasgn_sound. rewrite eval_comp. rewrite <- IHG. rewrite <- IHL.
+      * simpl. rewrite IHL. reflexivity.
+
 
 Theorem correctness : forall t G0 L0,
     Beval G0 L0 (pc t) = true ->
@@ -259,7 +291,6 @@ Proof.
         rewrite <- IHG. rewrite <- IHL. unfold Aeval_t. reflexivity.
 Qed.
 
-Ltac splits := repeat (try split).
 
 Lemma Gcomp_update_comm : forall G L x (v:Val) s,
     GComp G L (update s x (AConst v)) = update (GComp G L s) x v.
